proof: skeleton for `lambda`

theories/semantics.v
@@ -9,8 +9,8 @@ Require Import Unicode.Utf8.
 
 Require Import config.
 Require Import data_model.
+Require Import expression.
 Require Import finite_bags.
-Require Import formula.
 Require Import types.
 Require Import lattice.
 Require Import ordering.
@@ -19,1094 +19,139 @@ Require Import relation.
 Require Import util.
 
 Inductive project_list: Set :=
-  (* Denotes a "*" projection list. *)
+  (* Denotes a projection list that projects on *all*. *)
   | project_star: project_list
-  (*
-    Dentoes a project list consisting function applications, column names, and constants.
-    For example, if we have a schema `(IntegerType :: StringType :: BoolType :: nil)%type`,
-    then the following project list is valid:
-    ```
-    (simple_atomic_expression_func stf_id
-      (cons (simple_atomic_expression_column 0) nil)
-    )
-    ::
-    (simple_atomic_expression_func stf_id
-      (cons (simple_atomic_expression_column 1) nil)
-    )
-    ::
-    (simple_atomic_expression_func stf_id
-      (cons (simple_atomic_expression_column 2) nil)
-    )
-    ```
-
-    Elements in the projection list will be added with an explicit column name.
-  *)
-  | project: list (simple_atomic_expression * string) → project_list
+  (* Denotes a project list consisting of expressions, i.e., lambda terms. *)
+  | project: list (expression * string) → project_list
 .
 Hint Constructors project_list: core.
 
 (*
+  @param s The schema of the expression.
+  @param arg The expression for which the basic type is to be determined.
+  @param env The list of basic types that form the environment for the expression.
+  @returns option basic_type The basic type of the expression if it can be determined, `None` otherwise.
 
-  This function checks whether an expression is properly normalized. For an expression `expr`
-  to be normalized, it must satisfy the following conditions:
-  * If it is a function application, then either:
-    - The function contains only one argument and the argument is a column name, or
-    - The function contains more than one argument and all arguments are normalized.
-  * If it is a column name, then it is not normalized (because no identity function is applied).
-  * If it is a constant, then it is normalized.
-
-  Normalization is just ensure that each column is applied with a function so that we can easily
-  determine the basic type of the column as well as the label provenance of the column.
+  The `determine_bt_from_expr_helper` function is a recursive function that determines the basic type of an
+  expression given a schema and an environment of basic types. This function is used more like as a
+  type checker.
 *)
-Fixpoint normalized_expr (expr: simple_atomic_expression): Prop :=
-  match expr with
-  | simple_atomic_expression_column _ => False
-  | simple_atomic_expression_const _ _ => True
-  | simple_atomic_expression_func_unary _ expr' =>
-      match expr' with
-      | simple_atomic_expression_column _ => True
-      | simple_atomic_expression_const _ _ => True
-      | _ => normalized_expr expr'
-      end
-  | simple_atomic_expression_func_binary _ lhs rhs => normalized_expr lhs ∧ normalized_expr rhs
+Fixpoint determine_bt_from_expr_helper (s: schema) (arg: expression_lexed) (env: list expr_type):
+  option expr_type :=
+    match arg with
+    (* Lookup in the environment. *)
+    | expression_lexed_var n => nth_option env n
+    (* For constants, we already know its type. *)
+    | expression_lexed_const bt _ => Some (expr_type_basic bt)
+    (* For columns, we need to extract it from the schema. *)
+    | expression_lexed_column n =>
+        option_map (fun x => expr_type_basic x) (Tuple.nth_nocheck (♭ s) n)
+    (* For function abstraction, we encode the argument type, so wecan extract it and evaluate its body. *)
+    | expression_lexed_abs τ body =>
+        option_map (fun x => expr_type_func τ x) (determine_bt_from_expr_helper s body (τ :: env))
+    (* For function application, we need to evaluate the function and the argument and check if their types match. *)
+    | expression_lexed_app f x =>
+        match determine_bt_from_expr_helper s f env, determine_bt_from_expr_helper s x env with
+          | Some (expr_type_func τ1 τ2), Some τ3 =>
+            if expr_type_eqb τ1 τ3 then Some τ2 else None
+          | _, _ => None
+        end
+    (*
+      For binary operations, we need to evaluate the two arguments and check if their types match and
+      the operation type is correct.
+    *)
+    | expression_lexed_binary op x y =>
+        match determine_bt_from_expr_helper s x env, determine_bt_from_expr_helper s y env with
+          | Some τ1, Some τ2 =>
+            match op with
+              | binary_function op _ _ =>
+                match op with
+                | Arithmetic _ =>
+                  if expr_type_eqb τ1 (expr_type_basic IntegerType) then
+                    if expr_type_eqb τ2 (expr_type_basic IntegerType) then
+                      Some (expr_type_basic IntegerType)
+                    else None
+                  else None
+                | Comparison _ =>
+                  if expr_type_eqb τ1 τ2 then Some (expr_type_basic BoolType) else None
+                | Logical _ =>
+                  if expr_type_eqb τ1 (expr_type_basic BoolType) then
+                    if expr_type_eqb τ2 (expr_type_basic BoolType) then
+                      Some (expr_type_basic BoolType)
+                    else None
+                  else None
+              end
+            end
+          | _, _ => None
+        end
+    | expression_lexed_unary op x =>
+        match determine_bt_from_expr_helper s x env with
+          | Some τ =>
+            match op with
+              | unary_function op _ _ =>
+                match op with
+                | Not =>
+                  if expr_type_eqb τ (expr_type_basic BoolType) then
+                    Some (expr_type_basic BoolType)
+                  else None
+                | _ =>
+                  if expr_type_eqb τ (expr_type_basic IntegerType) then
+                    Some (expr_type_basic IntegerType)
+                  else None
+              end
+            end
+          | _ => None
+        end
+    | expression_lexed_agg op x =>
+        match determine_bt_from_expr_helper s x env with
+          | Some τ =>
+            match op with
+            | aggregate_function _ _ τ _ => Some (expr_type_basic τ)
+            end
+          | _ => None
+        end
+    end.
+
+Definition determine_bt_from_expr (s: schema) (arg: expression_lexed): option basic_type :=
+  match determine_bt_from_expr_helper s arg nil with
+    | Some (expr_type_basic bt) => Some bt
+    | _ => None
   end.
 
-Definition normalized (pl: project_list): Prop :=
+Fixpoint determine_schema (s: schema) (pl: list (expression * string)): option schema :=
   match pl with
-    | project_star => False
-    | project ℓ =>
-        (fix normalized' ℓ :=
-          match ℓ with
-          | nil => True
-          | (h, _) :: t => normalized_expr h ∧ normalized' t
+  | nil => Some nil
+  | (x, name) :: ℓ' =>
+    let lexed_expr := lex x nil in
+      match determine_bt_from_expr s lexed_expr with
+        | Some bt =>
+          match determine_schema s ℓ' with
+            | Some sch => Some ((bt, name) :: sch)
+            | None => None
           end
-        ) ℓ
-  end.
-
-(** 
-  @param s The schema, which is a list of attributes.
-  @param arg The simple atomic expression to evaluate.
-  @return An optional basic type that represents the type of the evaluated expression.
-
-  [bt_from_expr] is a function that takes a schema [s] and a simple atomic expression [arg], and returns an optional basic
-  type that represents the type of the evaluated expression.
-
-  The function works by pattern matching on the simple atomic expression [arg]. If [arg] is a column, it uses the [Tuple
-  nth_nocheck] function to get the type of the column from the schema. If [arg] is a constant, it simply returns the type of
-  the constant. If [arg] is a unary function, it recursively calls [determine_bt_from_expr] on the argument of the function.
-  If [arg] is a binary function, it recursively calls [determine_bt_from_expr] on both arguments of the function and checks if
-  their types match. If they do, it returns the type of the first argument. If they don't, it returns None.
-*)
-Fixpoint determine_bt_from_expr (s: schema) (arg: simple_atomic_expression): option basic_type :=
-  match arg with
-    | simple_atomic_expression_column c => Tuple.nth_nocheck (♭ s) c
-    | simple_atomic_expression_const bt _ => Some bt
-    | simple_atomic_expression_func_unary _ expr => determine_bt_from_expr s expr
-    | simple_atomic_expression_func_binary _ lhs rhs =>
-      match determine_bt_from_expr s lhs, determine_bt_from_expr s rhs with
-      | Some ty1, Some ty2 =>
-        if type_matches ty1 ty2 then Some ty1 else None
-      | _, _ => None
+        | None => None
       end
   end.
 
 (*
-  `determine_schema` is a function that takes a schema and a project list and returns a schema.
-  This function calculates the output schema for the project operation given the input schema
-  and the project list.
+  @param s The schema of the relation.
+  @return project_list The expanded project list.
 
-  * Note *
-  This project list must be first normalized.
-
-  For example, if we have a schema `(IntegerType :: StringType :: BoolType :: nil)%type` and
-  a project list `(simple_atomic_expression_column 0) :: (simple_atomic_expression_column 2) :: nil`,
-  then the result of `determine_schema` is `(IntegerType :: BoolType :: nil)%type`.
+  This function will expand `SELECT *` into its full project list.
 *)
-Definition determine_schema (s: schema) (pl: project_list): schema :=
-  match pl with
-    | project_star => s
-    | project ℓ =>
-        (fix determine ℓ :=
-          match ℓ with
-          | nil => nil
-          | (x, name) :: ℓ' => match x with
-                        | simple_atomic_expression_column c => 
-                          match Tuple.nth_nocheck (♭ s) c with
-                              | Some bt => (bt, name) :: determine ℓ'
-                              | None => determine ℓ'
-                            end
-                        | simple_atomic_expression_const bt _ => (bt, name) :: determine ℓ'
-                        | simple_atomic_expression_func_unary _ expr =>
-                          match determine_bt_from_expr s expr with
-                            | Some ty => (ty, name) :: determine ℓ'
-                            | None => determine ℓ'
-                            end
-                        | simple_atomic_expression_func_binary _ lhs rhs =>
-                          match determine_bt_from_expr s lhs, determine_bt_from_expr s rhs with
-                          | Some ty1, Some ty2 =>
-                            if type_matches ty1 ty2 then (ty1, name) :: determine ℓ' else determine ℓ'
-                          | _, _ => determine ℓ'
-                          end
-                      end
-          end) ℓ
-  end.
-
-Lemma determine_schema_length_le: ∀ s pl,
-  List.length (determine_schema s (project pl)) ≤ List.length pl.
-Proof.
-  induction pl.
-  - auto.
-  - apply Nat.lt_eq_cases in IHpl. destruct IHpl; destruct a.
-    + destruct s0.
-      * simpl in *. apply le_n_S. lia.
-      * simpl in *. destruct (Tuple.nth_nocheck (♭ s) n); try lia; auto.
-      * simpl in *. destruct (determine_bt_from_expr s s0); try lia; auto.
-      * simpl in *.
-        destruct (determine_bt_from_expr s s0_1); 
-        destruct (determine_bt_from_expr s s0_2);
-        try destruct (type_matches b0 b1); try lia; auto.
-    + destruct s0.
-      * simpl in *. lia.
-      * simpl in *. destruct (Tuple.nth_nocheck (♭ s) n).
-        -- simpl in *. apply le_n_S. lia.
-        -- simpl in *. lia.
-      * simpl in *. destruct (determine_bt_from_expr s s0).
-        -- simpl in *. apply le_n_S. lia.
-        -- simpl in *. lia.
-      * simpl in *. destruct (determine_bt_from_expr s s0_1);
-        destruct (determine_bt_from_expr s s0_2);
-        try destruct (type_matches b0 b1); simpl in *; lia.
-Qed.
-
-Lemma determine_schema_nil: ∀ s,
-  determine_schema s (project nil) = nil.
-Proof.
-  intros. simpl. auto.
-Qed.
-
-Lemma determine_schema_concat: ∀ s a ℓ,
-  determine_schema s (project (a :: @nil (simple_atomic_expression * string))) ++
-    determine_schema s (project ℓ) =
-  determine_schema s (project (a :: ℓ)).
-Proof.
-  induction a; induction a; auto; intros.
-  - simpl. destruct (Tuple.nth_nocheck (♭ s) n); auto.
-  - simpl. destruct (determine_bt_from_expr s a); auto.
-  - simpl. destruct (determine_bt_from_expr s a1);
-           destruct (determine_bt_from_expr s a2);
-           try destruct (type_matches b1 b2); auto.
-Qed.
-
-(** 
-  @param s The schema, which is a list of tuples where each tuple contains a type and a name.
-  @param n The starting index.
-  @return A list of tuples. Each tuple contains a simple atomic expression and a string.
-
-  [normalize_project_star] is a function that takes a schema [s] and a natural number [n], and returns a list of tuples. Each
-  tuple contains a simple atomic expression and a string.
-
-  The function works by iterating over the schema. For each attribute in the schema, it creates a new tuple. The first element of
-  the tuple is a simple atomic expression that represents the attribute's column in the relation, and the second element is the
-  attribute's name. The function uses the natural number [n] to keep track of the current column index. If the schema is empty,
-  it returns an empty list.
-*)
-Fixpoint normalize_project_star (s: schema) (n: nat): list (simple_atomic_expression * string) :=
-  match s with
+Definition project_all (s: schema): project_list :=
+  let f := fix f s n :=
+    match s with
     | nil => nil
-    | (_, name) :: s' =>
-      ((stf_id (simple_atomic_expression_column n)), name)
-          :: normalize_project_star s' (S n)
-  end.
+    | hd :: tl => (expression_column n, snd hd) :: f tl (S n)
+    end
+  in project (f s 0).
 
-(*
-  @param e The simple atomic expression to normalize.
-  @return The normalized simple atomic expression.
-
-  [normalize_expr] is a function that takes a simple atomic expression [e] and returns a normalized version of it.
-
-  The function works by pattern matching on the simple atomic expression [e]. If [e] is a column, it applies the Identity unary function to it. If [e] is a constant, it returns [e] as it is. If [e] is a unary function, it checks if the argument of the function is a column or a constant. If it is, it returns [e] as it is. If it's not, it recursively calls [normalize_expr] on the argument. If [e] is a binary function, it recursively calls [normalize_expr] on both arguments of the function.
-*)
-Fixpoint normalize_expr (e: simple_atomic_expression): simple_atomic_expression :=
-  match e with
-  | simple_atomic_expression_column c => 
-        (stf_id (simple_atomic_expression_column c))
-  | simple_atomic_expression_const _ _ => e
-  | simple_atomic_expression_func_unary f arg =>
-      match arg with
-        | simple_atomic_expression_column _ => e
-        | simple_atomic_expression_const _ _ => e
-        | _ => simple_atomic_expression_func_unary f (normalize_expr arg)
-      end
-  | simple_atomic_expression_func_binary f arg1 args2 =>
-      simple_atomic_expression_func_binary f (normalize_expr arg1) (normalize_expr args2)
-  end.
-
-(* 
-  `normalize_project_list_list` is a function that takes a schema and a list of simple atomic
-  expressions and returns a list of simple atomic expressions. The list of simple atomic
-  expressions is the same length as the schema.
-
-  This function converts from
-  - column names to function applications of the identity function to the column name,
-  - constants to constants, and
-  - functions to functions (by normalizing all its arguments).
-
-  We will later prove that this function preserves the semantics of the project operation.
-*)
-Fixpoint normalize_project_list_list
-  (s: schema) (pl: list (simple_atomic_expression * string)): list (simple_atomic_expression * string) :=
+Definition project_list_preprocess (s: schema) (pl: project_list): project_list :=
   match pl with
-    | nil => nil
-    | (e, name) :: pl' =>
-        let e' := (normalize_expr e) in (e', name) :: normalize_project_list_list s pl'
+    | project_star => project_all s
+    | _ => pl
   end.
-
-Lemma normalize_project_star_length: ∀ s n,
-  List.length (normalize_project_star s n) = List.length s.
-Proof.
-  induction s.
-  - auto.
-  - intros. simpl. destruct a.
-    specialize IHs with (n := S n). rewrite <- IHs. auto.
-Qed.
-
-Definition normalize_project_list (s: schema) (pl: project_list): project_list :=
-  project
-  (match pl with
-    | project_star => normalize_project_star s 0
-    | project ℓ => normalize_project_list_list s ℓ
-  end).
-
-Lemma normalize_preserve_length: ∀ s pl,
-  List.length pl = List.length (normalize_project_list_list s pl).
-Proof.
-  induction s; induction pl; try destruct a; try destruct a0; simpl; auto with *.
-Qed.
-
-Example sample_schema: schema :=
-  (IntegerType, "foo"%string) ::
-    (IntegerType, "bar"%string) ::
-      (IntegerType, "baz"%string) :: nil.
-Compute normalize_project_list sample_schema project_star.
-Compute normalize_project_list
-  sample_schema
-  (project
-    (((simple_atomic_expression_func_unary Lower
-      (simple_atomic_expression_column 0)
-    ), "foo"%string) :: nil)).
-
-Lemma normalize_star_normalized: ∀ s n, normalized (project (normalize_project_star s n)).
-Proof.
-  induction s.
-  - simpl. auto.
-  - intros. simpl.  destruct a.
-    specialize IHs with (n := S n).
-    simpl in IHs. auto. intuition. unfold normalized_expr. simpl. auto.
-Qed.
-
-Lemma normalized_cons: ∀ e pl, normalized (project (e :: pl)) →
-  normalized_expr (fst e) ∧ normalized (project pl).
-Proof.
-  induction pl; destruct e.
-  - simpl. auto.
-  - intros. simpl in *. intuition.
-Qed.
-
-Lemma normalized_implies_each_expr: ∀ ℓ,
-  normalized (project ℓ) →
-  ∀ e, List.In e ℓ → normalized_expr (fst e).
-Proof.
-  induction ℓ.
-  - intros. simpl in H0. inversion H0.
-  - intros. simpl in H0. intuition; destruct a.
-    + rewrite <- H1. simpl in H. intuition.
-    + apply IHℓ; auto.
-      simpl in H. intuition.
-Qed.
-
-Lemma normalized_list_cons: ∀ e ℓ,
-  normalized_expr (fst e) → normalized (project ℓ) → normalized (project (e :: ℓ)).
-Proof.
-  induction ℓ; destruct e.
-  - intros. simpl. auto.
-  - intros; destruct a.
-    apply normalized_cons in H0. intuition.
-    simpl. intuition.
-Qed.
-
-Lemma normalized_list_list_cons: ∀ s pl e,
-  normalized (project (normalize_project_list_list s (e :: pl))) →
-  normalized (project (normalize_project_list_list s pl)).
-Proof.
-  induction pl; destruct e.
-  - intros. simpl in *. auto.
-  - intros. simpl in *. intuition.
-Qed.
-
-Lemma normalize_expr_is_normalized: ∀ e, normalized_expr (normalize_expr e).
-Proof.
-  intros. subst. induction e; simpl; auto.
-  - induction e.
-    + simpl. auto.
-    + simpl. auto.
-    + induction e.
-      * simpl. auto.
-      * simpl. auto.
-      * intuition.
-      * intuition.
-    + induction e1; induction e2; intuition.
-Qed.
-
-Lemma normalize_is_normalized: ∀ s ℓ ℓ', ℓ' = (normalize_project_list s ℓ) → normalized ℓ'.
-Proof.
-  intros. subst. destruct ℓ.
-  - apply normalize_star_normalized.
-  - induction l.
-    + simpl. auto.
-    + simpl. destruct a.
-      intuition. apply normalize_expr_is_normalized.
-Qed.
-
-(* Some helper lemmas for manipulating dependent types. *)
-Section DtFacts.
-
-Lemma tuple_single_eq: ∀ ty, Tuple.tuple (♭ (ty :: nil)) = (prod (prod (type_to_coq_type (fst ty)) nat) unit).
-Proof.
-  intros. simpl. auto.
-  destruct ty.
-  simpl.
-  reflexivity.
-Qed.
-
-Lemma schema_const_ty_eq: ∀ expr ty c name s, expr = (simple_atomic_expression_const ty c, name) →
-  (ty, name) :: nil = determine_schema s (project (expr :: nil)).
-Proof.
-  intros.
-  destruct expr; inversion H; subst; intuition.
-Qed.
-
-Axiom nth_type_eq: ∀ s n (ok: n < List.length s) expr name, expr = simple_atomic_expression_column n →
-  nth s n ok :: nil = determine_schema s (project ((expr, name) :: nil)).
-
-(* By now, we can utilize `transport` or `eq_rect` to cast types: this is Leibniz equality. *)
-Example makes_no_sense: ∀ ty (r: relation (ty :: nil)) (t: list (prod (prod (type_to_coq_type (fst ty)) nat) unit)),
-  t = transport (tuple_single_eq ty) r.
-Admitted.
-
-End DtFacts.
-
-(*
-  @param s The schema, which is a list of tuples where each tuple contains a type and a name.
-  @param op The unary operation to be applied.
-  @param arg The simple atomic expression to evaluate.
-  @param name The name of the attribute.
-  @return A proposition that asserts the type of the evaluated expression remains the same when a
-          unary function is applied.
-=
-  [unary_function_preserves_type] is a lemma that asserts that applying a unary function [op] to a
-  simple atomic expression [arg] does not change the type of the evaluated expression. This is
-  demonstrated by showing that the schema determined by projecting the evaluated expression with the
-  unary function applied is the same as the schema determined by projecting the evaluated expression
-  without the unary function applied.
-*)
-Lemma unary_function_preserves_type: ∀ s op arg name,
-  (determine_schema s (project (
-    (simple_atomic_expression_func_unary op arg, name) :: nil
-  ))) =
-  (determine_schema s (project (<< (arg); (name) >> :: nil))).
-Proof.
-  intros. simpl.
-  destruct (determine_bt_from_expr s arg) eqn: Heq; destruct arg eqn: Harg.
-  - inversion Heq. subst. reflexivity.
-  - inversion Heq. subst. simpl in *.
-    destruct (Tuple.nth_nocheck (♭ s)).
-    + inversion Heq. subst. reflexivity.
-    + inversion Heq.
-  - destruct (determine_bt_from_expr s s0) eqn: Heq'.
-    + simpl in *.
-      assert (Some b = Some b0).
-      {
-        eapply trans_eq. symmetry in Heq. eauto. eauto.
-      }
-      inversion H. subst. reflexivity.
-    + assert (Some b = None).
-      {
-        eapply trans_eq. symmetry in Heq. eauto. eauto.
-      }
-      inversion H.
-  - inversion Heq.
-    destruct (determine_bt_from_expr s s0_1) eqn: Heq1;
-    destruct (determine_bt_from_expr s s0_2) eqn: Heq2.
-    try destruct (type_matches b1 b2) eqn: Heq3; inversion H0.
-    + apply type_matches_eq in Heq3. subst. inversion H0. reflexivity.
-    + inversion H0.
-    + inversion H0.
-    + inversion H0.
-  - inversion Heq.
-  - inversion Heq. rewrite H0. reflexivity.
-  - inversion Heq. rewrite H0. reflexivity.
-  - inversion Heq.
-    destruct (determine_bt_from_expr s s0_1) eqn: Heq1;
-    destruct (determine_bt_from_expr s s0_2) eqn: Heq2;
-    try destruct (type_matches b0 b1) eqn: Heq3; try inversion H0; reflexivity.
-Defined.
-
-Lemma unary_function_preserves_type': ∀ expr s op arg name,
-  expr = (simple_atomic_expression_func_unary op arg, name) →
-  (determine_schema s (project (expr :: nil))) =
-  (determine_schema s (project (<< (arg); (name) >> :: nil))).
-Proof.
-  intros. subst. apply unary_function_preserves_type.
-Qed.
-
-Fixpoint determine_agg_schema (al: agg_list): schema.
-  refine (
-    match al with
-      | nil => nil
-      | (cur, name) :: tl => _
-    end
-  ).
-Admitted.
-
-Example determine_agg_schema_correct: determine_agg_schema
-  ((((Count, (aggregate_function IntegerType IntegerType (fun x y => x + y)), 0)), "foo"%string) :: (((Count, (aggregate_function IntegerType IntegerType (fun x y => x + y)), 0)), "foo"%string) :: nil) =
-  (IntegerType, "foo"%string) :: (IntegerType, "foo"%string) :: nil.
-Proof. reflexivity. Qed.
-
-
-Inductive operator: Type :=
-  | operator_empty: operator
-  (* `nat` means the index of the relation it wants to access inside `db`. *)
-  | operator_relation: nat → operator
-  | operator_union: operator → operator → operator
-  | operator_join: operator → operator → operator
-  | operator_project: project_list → operator → operator
-  | operator_select: ∀ s, formula (♭ s) → operator → operator
-  | operator_groupby_having: ∀ s, groupby_list → agg_list → formula s → operator → operator
-.
-
-(*
-  @param s The schema, which is a list of tuples where each tuple contains a type and a name.
-  @param n The length of the relation to be created.
-  @param t The tuple to be repeated.
-  @return A relation of length [n] where each tuple is [t].
-
-  [tuple_of_length_n] returns a relation of length [n] where each tuple is [t]. The function
-  works by recursively appending [t] to the relation until it reaches the desired length.
-*)
-Fixpoint tuple_of_length_n s (n: nat) (t: Tuple.tuple (♭ s)): relation s :=
-match n with
-  | O => nil
-  | S n' => t :: tuple_of_length_n s n' t
-  end.
-
-Definition get_new_policy cur op: Policy.policy :=
-  match cur with
-  | ∎ => cur
-  | ℓ ⇝ p =>
-    match Policy.can_declassify_dec ℓ op with
-    | left _ => p
-    | right _ => cur
-    end
-  end.
-
-(*
-  @param bt The base type of the cell.
-  @param f_type The type of the unary function.
-  @param f The unary function to be applied.
-  @param arg A tuple containing the cell value and its index.
-  @param Γ The policy context.
-  @param p The provenance context.
-  @return An optional tuple containing the result of applying the unary function to the cell
-          value, the updated policy context, and the updated provenance context.
-
-  This function applies a unary function to a cell in a relation. If the unary function can
-  be successfully applied, it returns a tuple containing the result of the function applica-
-  tion, the updated policy context, and the updated provenance context. If the unary function
-  cannot be applied (for example, if the function is not defined for the base type of the
-  cell), the function returns `None`.
-*)
-Inductive apply_unary_function_in_cell bt:
-  UnOp → unary_func → (type_to_coq_type bt * nat) → Policy.context → prov_ctx
-       → option (type_to_coq_type bt * Policy.context * prov_ctx) → Prop :=
-  | E_LabelNotFound: ∀ op f arg Γ p,
-      label_lookup Γ (snd arg) = None ∨
-      label_lookup p (snd arg) = None →
-      apply_unary_function_in_cell bt op f arg Γ p None
-  | E_PolicyErr: ∀ op f arg Γ p p_cur p_f,
-      label_lookup Γ (snd arg) = Some p_cur →
-      p_f = ∘ (Policy.policy_transform ((unary_trans_op op) :: nil)) →
-      ¬ (p_cur ⪯ p_f) →
-      apply_unary_function_in_cell bt op f arg Γ p None
-  | E_PolicyOk: ∀ op f lambda arg Γ p p_cur prov_cur p_new prov_new ℓ p_f res Γ' p',
-      label_lookup Γ (snd arg) = Some p_cur →
-      label_lookup p (snd arg) = Some prov_cur →
-      ℓ = (Policy.policy_transform ((unary_trans_op op) :: nil)) →
-      p_f = (∘ ℓ) →
-      p_cur ⪯ p_f →
-      p_new = get_new_policy p_cur ℓ →
-      prov_new = prov_list (prov_trans_unary op) ((snd arg, prov_cur) :: nil) →
-      f = (unary_function bt lambda) →
-      lambda (fst arg) = res →
-      Γ' = update_label Γ (snd arg) p_new →
-      p' = update_label p (snd arg) prov_new →
-      apply_unary_function_in_cell bt op f arg Γ p (Some (res, Γ', p'))
-.
-
-(*
-  @param ty An attribute containing a type and a name.
-  @param r The relation, which is a list of tuples where each tuple contains a single type.
-         Somehow we must calculate the type of `r`.
-  @param Γ The policy context.
-  @param p The proof context.
-  @return An optional tuple containing the relation, the policy context, and the proof context.
-
-  This function does the actual function application on a relation containing only one column on
-  which the unary function should be applied.
-*)
-Inductive do_apply_unary_function (ty: Attribute) (r: relation (ty :: nil)):
-  UnOp → unary_func → Policy.context → prov_ctx
-       → option (relation (ty :: nil) * Policy.context * prov_ctx) → Prop :=
-  | E_EmptyRelation: ∀ op f Γ p,
-      r = nil →
-      do_apply_unary_function ty r op f Γ p (Some (nil, Γ, p))
-  | E_ApplyError: ∀ op f arg id tl Γ p,
-      (tuple_single_eq ty) ♯ r = [[ (arg, id) ]] :: tl →
-      apply_unary_function_in_cell (fst ty) op f (arg, id) Γ p None →
-      do_apply_unary_function ty r op f Γ p None
-   | E_ApplyErrorTail: ∀ op f arg id tl Γ p,
-      (tuple_single_eq ty) ♯ r = [[ (arg, id) ]] :: tl →
-      do_apply_unary_function ty (eq_sym (tuple_single_eq ty) ♯ tl) op f Γ p None →
-      do_apply_unary_function ty r op f Γ p None
-  | E_ApplyOk: ∀ op f arg id tl tl' Γ p ret Γ1 Γ2 p1 p2 res,
-      (tuple_single_eq ty) ♯ r = [[ (arg, id) ]] :: tl →
-      apply_unary_function_in_cell (fst ty) op f (arg, id) Γ p (Some (ret, Γ1, p1)) →
-      (* Since this operation is sequential, we can just feed the updated env to cons. *)
-      do_apply_unary_function ty (eq_sym (tuple_single_eq ty) ♯ tl) op f Γ1 p1 (Some (tl', Γ2, p2)) →
-      res = (Some (eq_sym (tuple_single_eq ty) ♯ ([[ (ret, id) ]] ::
-                  ((tuple_single_eq ty) ♯ tl')),
-                  Γ2, p2)) →
-      do_apply_unary_function ty r op f Γ p res
-.
-
-(*
-  @param ty An attribute containing a type and a name.
-  @param op The unary operation to be applied.
-  @param ok A proof that the length of the schema [s] is 1.
-  @param ctx A tuple containing the relation, the policy context, and the proof context.
-  @return An optional tuple containing the relation, the policy context, and the proof context
-          after applying the unary operation.
-
-  [apply_unary_function_in_relation] is a function that takes a schema [s], a unary operation
-  [op], a proof [ok] that the length of the schema is 1, and a context [ctx] that contains the
-  relation, the policy context, and the proof context. It applies the unary operation [op] to
-  the relation in the context and returns an optional tuple containing the updated relation,
-  policy context, and proof context. If the operation cannot be applied, it returns None.
-
-  This is just an entrypoint for the actual function [do_apply_unary_function].
-*)
-Inductive apply_unary_function_in_relation ty (r: relation (ty :: nil)):
-  UnOp → Policy.context → prov_ctx → 
-    option (relation (ty :: nil) * Policy.context * prov_ctx) → Prop :=
-  | E_ApplyEmptyRelation: ∀ op Γ p,
-      r = nil →
-      apply_unary_function_in_relation ty r op Γ p None
-  | E_ApplyIdentity: ∀ op r' tp tp_tl Γ Γ' p p',
-      r = tp :: tp_tl →
-      op = Identity →
-      do_apply_unary_function ty r op (unary_function (fst ty) (fun x => x)) Γ p (Some (r', Γ', p')) →
-      apply_unary_function_in_relation ty r op Γ p (Some (r', Γ', p'))
-  (* Others are not defined. *)
-.
-
-(*
-  @param s The schema of the relation.
-  @param r The relation, which is a list of tuples where each tuple corresponds to a row in the relation.
-  @param expr A tuple containing a simple atomic expression and a string. The simple atomic expression
-              represents a column in the relation, and the string is the name of the column.
-  @param Policy.context The policy context.
-  @param prov_ctx The proof context.
-  @return An optional tuple containing the relation, the policy context, and the proof context.
-*)
-Inductive apply_proj_elem s (r: relation s) (expr: simple_atomic_expression * string):
-  Policy.context → prov_ctx →
-    option (relation (determine_schema s (project (expr :: nil))) * basic_type * Policy.context * prov_ctx) → Prop :=
-    (* We forbid directly reading from a column; this may violate the security policy. *)
-  | E_ApplyColumn: ∀ Γ p n name
-                  (case_column: expr = (simple_atomic_expression_column n, name)),
-
-        apply_proj_elem s r expr Γ p None
-    (* If we are doing projection of constants, we directly construct a column without any modification. *)
-  | E_ApplyConst: ∀ Γ p ty val name res
-                 (case_expr: expr = (simple_atomic_expression_const ty val, name)),
-
-        let res_tmp := (tuple_of_length_n ((ty, name) :: nil) (List.length r) ((val, 0), tt)) in
-          (* A transportation for type casting. *)
-          res = (schema_const_ty_eq expr ty val name s case_expr ♯ res_tmp) →
-          apply_proj_elem s r expr Γ p (Some (res, ty, Γ, p))
-  | E_ApplyUnaryFunctionColumnError: ∀ Γ p op arg n name 
-                          (case_expr: expr = (simple_atomic_expression_func_unary op arg, name)),
-
-        arg = (simple_atomic_expression_column n) →
-        n >= List.length s →
-        apply_proj_elem s r expr Γ p None
-  | E_ApplyUnaryFunctionColumnError2: ∀ Γ p op arg n (ok: n < List.length s) name tuples 
-                          (case_expr: expr = (simple_atomic_expression_func_unary op arg, name))
-                          (case_arg: arg = (simple_atomic_expression_column n)),
-        tuples = extract_column s r n ok →
-        apply_unary_function_in_relation _ tuples op Γ p None →
-        apply_proj_elem s r expr Γ p None
-  | E_ApplyUnaryFunctionColumnOk: ∀ Γ p op arg n (ok: n < List.length s) name tuples res_tmp res_tmp' res Γ' p'
-                          (case_expr: expr = (simple_atomic_expression_func_unary op arg, name))
-                          (case_arg: arg = (simple_atomic_expression_column n)),
-
-        tuples = extract_column s r n ok →
-        apply_unary_function_in_relation _ tuples op Γ p (Some (res_tmp, Γ', p')) →
-        res_tmp' = (nth_type_eq s n ok arg name case_arg ♯ res_tmp) →
-        (* Do a type casting. *)
-        res = (eq_sym (unary_function_preserves_type' expr s op arg name case_expr) ♯ res_tmp') →
-        apply_proj_elem s r expr Γ p (Some (res, (fst (nth s n ok)), Γ', p'))
-  | E_ApplyUnaryFunctionOtherOk: ∀ Γ Γ' Γ'' p p' p'' op arg ty1 ty2 n name arg' res_tmp res
-                            (case_expr: expr = (simple_atomic_expression_func_unary op arg, name))
-                            (* We can prove this later. *)
-                            (type_matches: determine_schema s (project (<< (arg); (name) >> :: nil)) = (ty1 :: nil)),
-        arg ≠ (simple_atomic_expression_column n) →
-        (* We first recursively evaluate the argument. *)
-        apply_proj_elem s r (arg, name) Γ p (Some (arg', ty2, Γ', p')) →
-        (fst ty1) = ty2 →
-        (* Then we apply the unary function to the argument. *)
-        apply_unary_function_in_relation _ (type_matches ♯ arg') op Γ' p' (Some (res_tmp, Γ'', p'')) →
-        res = (eq_sym (unary_function_preserves_type' expr s op arg name case_expr) ♯ (eq_sym type_matches ♯ res_tmp)) →
-        apply_proj_elem s r expr Γ p (Some (res, ty2, Γ'', p''))
-  | E_ApplyUnaryFunctionOtherErr1: ∀ Γ p op arg n name
-                            (case_expr: expr = (simple_atomic_expression_func_unary op arg, name)),
-        arg ≠ (simple_atomic_expression_column n) →
-        (* We first recursively evaluate the argument. *)
-        apply_proj_elem s r (arg, name) Γ p None →
-        apply_proj_elem s r expr Γ p None
-  | E_ApplyUnaryFunctionOtherNoSchema: ∀ Γ p op arg n name
-                            (case_expr: expr = (simple_atomic_expression_func_unary op arg, name)),
-                            (* We can prove this later. *)
-        determine_bt_from_expr s arg = None →
-        arg ≠ (simple_atomic_expression_column n) →
-        apply_proj_elem s r expr Γ p None
-  | E_ApplyUnaryFunctionOtherErr2: ∀ Γ Γ' p p' op arg ty1 ty2 n name arg'
-                            (case_expr: expr = (simple_atomic_expression_func_unary op arg, name))
-                            (* We can prove this later. *)
-                            (type_matches: determine_schema s (project (<< (arg); (name) >> :: nil)) = (ty1 :: nil)),
-        arg ≠ (simple_atomic_expression_column n) →
-        (* We first recursively evaluate the argument. *)
-        apply_proj_elem s r (arg, name) Γ p (Some (arg', ty2, Γ', p')) →
-        apply_unary_function_in_relation _ (type_matches ♯ arg') op Γ' p' None →
-        apply_proj_elem s r expr Γ p None
-  | E_ApplyUnaryFunctionOtherTypeMismatch: ∀ Γ Γ' p p' op arg ty1 ty2 n name arg'
-                            (case_expr: expr = (simple_atomic_expression_func_unary op arg, name))
-                            (* We can prove this later. *)
-                            (type_matches: determine_schema s (project (<< (arg); (name) >> :: nil)) = (ty1 :: nil)),
-        arg ≠ (simple_atomic_expression_column n) →
-        (* We first recursively evaluate the argument. *)
-        apply_proj_elem s r (arg, name) Γ p (Some (arg', ty2, Γ', p')) →
-        (fst ty1) ≠ ty2 →
-        apply_proj_elem s r expr Γ p None
-  | E_Nonimplemented: ∀ Γ p op arg1 arg2 name
-                     (case_expr: expr = (simple_atomic_expression_func_binary op arg1 arg2, name)),
-      apply_proj_elem s r expr Γ p None
-  .
-
-(*
-  @param s The schema of the relation.
-  @param r The relation, which is a list of tuples where each tuple contains a single type.
-  @param ℓ A list of simple atomic expressions and their corresponding string identifiers.
-  @param Policy.context The policy context.
-  @param prov_ctx The proof context.
-  @return An optional tuple containing the relation, the policy context, and the proof context.
-
-  This function applies a projection operation to a relation. The projection operation is specified by the list of
-  simple atomic expressions `ℓ`. Each simple atomic expression in `ℓ` represents a column in the relation `r` that
-  should be included in the result. The function returns an optional value. If the projection operation can be
-  successfully applied, the function returns `Some` with a tuple containing the resulting relation, the updated
-  policy context, and the updated proof context. If the projection operation cannot be applied (for example, if a
-  simple atomic expression in `ℓ` does not correspond to a column in `r`), the function returns `None`.
-*)
-Inductive apply_proj_in_relation s (r: relation s) (ℓ: list (simple_atomic_expression * string)):
-  Policy.context → prov_ctx → 
-    option (relation (determine_schema s (project ℓ)) * Policy.context * prov_ctx) → Prop :=
-  (* We do not accept lists that are not normalized. *)
-  | E_Unnormalized: ∀ Γ p,
-      ¬ (normalized (project ℓ)) →
-      apply_proj_in_relation s r ℓ Γ p None
-  | E_ApplyElemEmpty: ∀ Γ p,
-      ℓ = nil ∨ r = nil →
-      apply_proj_in_relation s r ℓ Γ p (Some (nil, Γ, p))
-  | E_ApplyElemErrHead: ∀ Γ p hd tl (proj_case: ℓ = hd :: tl),
-      r ≠ nil →
-      apply_proj_elem s r hd Γ p None →
-      apply_proj_in_relation s r ℓ Γ p None
-  | E_ApplyElemErrTail: ∀ hd hd' Γ Γ' p p' tl (proj_case: ℓ = hd :: tl),
-      r ≠ nil →
-      apply_proj_elem s r hd Γ p (Some (hd', Γ', p')) →
-      apply_proj_in_relation s r tl Γ' p' None →
-      apply_proj_in_relation s r ℓ Γ p None
-  | E_ApplyElemOk: ∀ Γ Γ' Γ'' p p' p'' hd hd' tl tl' col
-                (proj_case: ℓ = hd :: tl),
-      r ≠ nil →
-      apply_proj_elem s r hd Γ p (Some (hd', Γ', p')) →
-      apply_proj_in_relation s r tl Γ' p' (Some (tl', Γ'', p'')) →
-      (*
-        Goal:
-        (determine_schema s (project (hd :: nil)) ++
-        determine_schema s (project tl)) = determine_schema s (project ℓ)
-        -------------------------------
-        project ℓ = project (hd :: tl) by ℓ = hd :: tl with ♯
-        --–----------------------------
-        Then by determine_schema_concat we have:
-        (determine_schema s (project (hd :: nil)) ++
-        determine_schema s (project tl)) = determine_schema s (project (hd :: tl))
-        -------------------------------
-      *)
-      let col_tmp := (relation_product _ _ (fst hd') tl') in
-        let col_proxy := ((determine_schema_concat s hd tl) ♯ col_tmp) in
-          col = ((eq_sym proj_case) ♯ col_proxy) →
-          apply_proj_in_relation s r ℓ Γ p (Some (col, Γ'', p''))
-.
-
-Lemma apply_unary_function_in_relation_terminate: ∀ s r op Γ p,
-  ∃ res, apply_unary_function_in_relation s r op Γ p res.
-Proof.
-Admitted.
-
-Lemma apply_proj_elem_terminate: ∀ s r expr Γ p, ∃ res,
-  apply_proj_elem s r expr Γ p res.
-Proof.
-  intros s r expr.
-  refine (
-    match expr with
-    | (exp, name) =>
-        (*
-          The trick is to split the tuple into just its left part to pass the termination checker.
-
-          This is because reducing *only* the left part of the tuple will not convince Coq that
-          the function will terminate; but we do not use the right part, so we just throw it away
-          and do not use it as a principle argument of recursion. 
-        *)
-        (fix proof e :=
-          match e as e' return e = e' → _ with 
-            | simple_atomic_expression_const ty val => _
-            | simple_atomic_expression_column n => _
-            | _ => _
-          end eq_refl) exp
-    end); intros.
-  - pose (res := (schema_const_ty_eq (simple_atomic_expression_const ty val, name) ty val name s eq_refl ♯
-      tuple_of_length_n (<< (ty); (name) >> :: nil) (Datatypes.length r) (val, 0, tt))).
-    subst. exists (Some (res, ty, Γ, p)).
-
-    eapply E_ApplyConst with (val := val) (name := name) (case_expr := eq_refl); eauto.
-  - exists None. eapply E_ApplyColumn; eauto.
-  - specialize proof with (e := s0) (Γ := Γ) (p := p).
-    destruct proof.
-    destruct x.
-    + (* Some *)
-      destruct p0 as [ [ [ r' ty ] Γ'] p'].
-      destruct s0.
-      * destruct (apply_unary_function_in_relation_terminate _ (eq_refl ♯ r') u Γ' p').
-       (* destructing the nested evaluation. *)
-       destruct x.
-       -- (* Some *)
-         destruct p0 as [ [ r'' Γ'' ] p''].
-         destruct (basic_type_eq_dec ty bt).
-         ++ simpl in *. specialize E_ApplyUnaryFunctionOtherOk with
-                (expr := (simple_atomic_expression_func_unary u (simple_atomic_expression_const bt t), name))
-                (case_expr := eq_refl)
-                (ty1 := (bt, name))
-                (ty2 := ty)
-                (n := 0)
-                (res_tmp := r'').
-            intros.
-            exists (Some (((eq_sym (unary_function_preserves_type' 
-              (simple_atomic_expression_func_unary u (simple_atomic_expression_const bt t), name) s u
-                (simple_atomic_expression_const bt t) name eq_refl) ♯ (eq_sym eq_refl ♯ r''))),
-                  ty, Γ'', p'')).
-            eapply H2; eauto.
-            ** red. intros. discriminate.
-            ** simpl in *. auto.
-
-        ++ (* Type mismatch! *)
-          exists None. eapply E_ApplyUnaryFunctionOtherTypeMismatch with (ty1 := (bt, name)) (n := 0); eauto.
-          red. intros. discriminate.
-      -- (* None *)
-          exists None. eapply E_ApplyUnaryFunctionOtherErr2 with (n := 0); eauto.
-          red. intros. discriminate.
-      * (* This happens when the inner argument is a column type. *)
-         destruct (lt_dec n (List.length s)) as [ok | not_ok]. 
-         -- pose (tuple := extract_column s r n ok).
-            destruct (apply_unary_function_in_relation_terminate _ tuple u Γ p).
-            destruct x as [ [ [res_tmp Γ_tmp ] p_tmp ] | ].
-            ++ (* Some *)
-               pose ((nth_type_eq s n ok (simple_atomic_expression_column n) name eq_refl) ♯ res_tmp) as res_tmp'.
-               pose (eq_sym (unary_function_preserves_type' (simple_atomic_expression_func_unary u (simple_atomic_expression_column n), name) s u (simple_atomic_expression_column n) name eq_refl) ♯ res_tmp') as res.
-               exists (Some (res, (fst (nth s n ok)), Γ_tmp, p_tmp)).
-               eapply E_ApplyUnaryFunctionColumnOk with (tuples := tuple) (n := n) (arg := simple_atomic_expression_column n)(ok := ok) (res_tmp := res_tmp) (res_tmp' := res_tmp') (case_arg := eq_refl) (case_expr := eq_refl); eauto.
-            ++ exists None. eapply E_ApplyUnaryFunctionColumnError2 with (n := n); eauto.
-          -- exists None. eapply E_ApplyUnaryFunctionColumnError with (n := n); eauto. lia.
-      * 
-      (* Let us again use dependent pattern matching. *)
-        refine (
-          match determine_bt_from_expr s s0 as t return t = determine_bt_from_expr s s0 -> _ with
-            | None => _
-            | Some ty => _
-          end eq_refl
-        ); intros.
-        -- assert (<< ty ; name >> :: nil = determine_schema s (
-              project (<< (simple_atomic_expression_func_unary u 
-                (simple_atomic_expression_func_unary u0 s0)); (name) >> :: nil))).
-          {
-            simpl. rewrite <- H1. reflexivity.
-          }
-          (* Now this tactic type-checks. *)
-          destruct (apply_unary_function_in_relation_terminate _ (eq_sym H2 ♯ r') u Γ' p').
-          destruct x as [ [ [res_tmp Γ_tmp ] p_tmp ] | ].
-          ++ (* Transport the type to make Coq happy. *)
-            destruct (basic_type_eq_dec ty ty0).
-            (* Π (A: U) Π (a b: A) (a = b) → P (a) -> P(b) *)
-            ** exists (Some ((eq_sym (unary_function_preserves_type'
-                  (simple_atomic_expression_func_unary u (simple_atomic_expression_func_unary u0 s0), name) s u
-                    (simple_atomic_expression_func_unary u0 s0) name eq_refl) ♯ (H2 ♯ res_tmp)),
-                      ty, Γ_tmp, p_tmp)).
-             eapply E_ApplyUnaryFunctionOtherOk with (n := 0) (case_expr := eq_refl); eauto.
-              --- red. intros. discriminate.
-              --- subst. auto.
-              --- auto.
-              --- rewrite eq_sym_involutive. auto.
-           ** exists None. eapply E_ApplyUnaryFunctionOtherTypeMismatch; eauto. instantiate (1 := 0).
-              red. intros. discriminate.
-          ++ exists None. eapply E_ApplyUnaryFunctionOtherErr2 with (n := 0); eauto.
-              red. intros. discriminate.
-        -- exists None. eapply E_ApplyUnaryFunctionOtherNoSchema with (n := 0); eauto.
-           red. intros. discriminate.
-      * refine (
-          match determine_bt_from_expr s s0_1 as ty1', determine_bt_from_expr s s0_2 as ty2'
-            return determine_bt_from_expr s s0_1 = ty1' → determine_bt_from_expr s s0_2 = ty2' → _
-          with
-          | Some ty1, Some ty2 =>
-            match type_matches ty1 ty2 as bt return type_matches ty1 ty2 = bt → _ with
-            | true => _
-            | false => _
-            end eq_refl
-          | _, _ => _
-          end eq_refl eq_refl
-        ); intros.
-        -- assert (determine_schema s (project ((simple_atomic_expression_func_binary b s0_1 s0_2, name) :: nil)) = << ty1 ; name >> :: nil).
-        {
-          simpl. rewrite H2. rewrite H3. rewrite H1. reflexivity.
-        }
-        destruct (apply_unary_function_in_relation_terminate _ (H4 ♯ r') u Γ' p').
-        destruct x as [ [ [res_tmp Γ_tmp ] p_tmp ] | ].
-          ++ destruct (basic_type_eq_dec ty ty1).
-            ** exists (Some ((eq_sym (unary_function_preserves_type'
-                  (simple_atomic_expression_func_unary u (simple_atomic_expression_func_binary b s0_1 s0_2), name) s u
-                    ((simple_atomic_expression_func_binary b s0_1 s0_2)) name eq_refl) ♯ (eq_sym H4 ♯ res_tmp)),
-                      ty, Γ_tmp, p_tmp)).
-               eapply E_ApplyUnaryFunctionOtherOk with (n := 0) (case_expr := eq_refl); eauto.
-               --- red. intros. discriminate.
-               --- subst. auto.
-            ** exists None. eapply E_ApplyUnaryFunctionOtherTypeMismatch; eauto. instantiate (1 := 0).
-               red. intros. discriminate.
-         ++ exists None. eapply E_ApplyUnaryFunctionOtherErr2 with (n := 0); eauto.
-              red. intros. discriminate.
-        -- exists None. eapply E_ApplyUnaryFunctionOtherNoSchema; eauto. 
-           simpl. rewrite H2. rewrite H3. rewrite H1. reflexivity. instantiate (1 := 0).
-           red. intros. discriminate.
-        -- exists None. eapply E_ApplyUnaryFunctionOtherNoSchema; eauto. 
-           simpl. rewrite H2. rewrite H1. reflexivity. instantiate (1 := 0).
-           red. intros. discriminate.
-        -- exists None. eapply E_ApplyUnaryFunctionOtherNoSchema; eauto. 
-           simpl. rewrite H1. reflexivity. instantiate (1 := 0).
-           red. intros. discriminate.
-    + (* None *)
-      destruct s0.
-      * exists None. eapply E_ApplyUnaryFunctionOtherErr1; eauto. simpl.
-        instantiate (1 := 0). red. intros. discriminate.
-      * (* `apply_proj_elem` has nothing to do with f(c); we just need to dicuss this case alone. *)
-        destruct (lt_dec n (List.length s)) as [ok | not_ok].
-        -- pose (tuple := extract_column s r n ok).
-           destruct (apply_unary_function_in_relation_terminate _ tuple u Γ p).
-           destruct x as [ [ [res_tmp Γ_tmp ] p_tmp ] | ].
-           ++ pose ((nth_type_eq s n ok (simple_atomic_expression_column n) name eq_refl) ♯ res_tmp) as res_tmp'.
-               pose (eq_sym (unary_function_preserves_type' (simple_atomic_expression_func_unary u (simple_atomic_expression_column n), name) s u (simple_atomic_expression_column n) name eq_refl) ♯ res_tmp') as res.
-               exists (Some (res, (fst (nth s n ok)), Γ_tmp, p_tmp)).
-               eapply E_ApplyUnaryFunctionColumnOk with (tuples := tuple) (n := n) (arg := simple_atomic_expression_column n)(ok := ok) (res_tmp := res_tmp) (res_tmp' := res_tmp') (case_arg := eq_refl) (case_expr := eq_refl); eauto.
-            ++ exists None. eapply E_ApplyUnaryFunctionColumnError2 with (n := n); eauto.
-        -- exists None. eapply E_ApplyUnaryFunctionColumnError with (n := n); eauto. lia.
-      * exists None. eapply E_ApplyUnaryFunctionOtherErr1; eauto. simpl.
-        instantiate (1 := 0). red. intros. discriminate.
-      * exists None. eapply E_ApplyUnaryFunctionOtherErr1; eauto. simpl.
-        instantiate (1 := 0). red. intros. discriminate.
-  - exists None. apply E_Nonimplemented with (op := b) (arg1 := s0) (arg2 := s1) (name := name); eauto.
-Qed.
-
-Lemma apply_proj_in_relation_terminate: ∀ s r ℓ Γ p,
-  ∃ res, apply_proj_in_relation s r ℓ Γ p res.
-Proof.
-  intros s r.
-  destruct r.
-  - intros. exists (Some (nil, Γ, p)). econstructor; eauto.
-  - refine (
-    fix proof ℓ Γ p :=
-      (*
-        Interestingly `induction n eqn: H` tactic messes up the dependent variables;
-        we instead use refine to do the induction.
-      *)
-      match ℓ as ℓ' return ℓ = ℓ' → _ with
-      | nil => fun _ => _
-      | hd :: tl => fun _ => _
-      end eq_refl
-  ).
-    + exists (Some (nil, Γ, p)). econstructor; eauto.
-    + destruct (apply_proj_elem_terminate s (t :: r) hd Γ p).
-      destruct x as [ [ [r' Γ'] p' ] |] eqn: Hx1.
-      * specialize proof with (ℓ := tl) (Γ := Γ') (p := p').
-        destruct proof.
-        destruct x0 as [ [ [r'' Γ''] p''] |] eqn: Hx2.
-        -- pose (col := (eq_sym eq_refl ♯
-                        (determine_schema_concat s hd tl ♯
-                          relation_product (determine_schema s (project (hd :: nil)))
-                              (determine_schema s (project tl)) (fst r') r''))).
-          exists (Some (col, Γ'', p'')).
-          specialize E_ApplyElemOk with (r := (t :: r)) (ℓ := ℓ) (hd := hd) (tl := tl) (hd' := r') (tl' := r'') (Γ := Γ) (Γ' := Γ') (Γ'' := Γ'') (p := p) (p' := p') (p'' := p'') (proj_case := e).
-          intros. subst.
-          eapply H1; eauto. red. intros. discriminate.
-        -- exists None. eapply E_ApplyElemErrTail; eauto. red. intros. discriminate.
-      * exists None. eapply E_ApplyElemErrHead; eauto. red. intros. discriminate.
-Qed.
-
-Lemma apply_proj_elem_deterministic: ∀ s r expr Γ p res1 res2,
-  apply_proj_elem s r expr Γ p res1 →
-  apply_proj_elem s r expr Γ p res2 →
-  res1 = res2.
-Proof.
-Admitted.
-
-Lemma apply_proj_in_relation_deterministic: ∀ s r ℓ Γ p res1 res2,
-  normalized (project ℓ) →
-  apply_proj_in_relation s r ℓ Γ p res1 →
-  apply_proj_in_relation s r ℓ Γ p res2 →
-  res1 = res2.
-Proof.
-  induction ℓ; intros; inversion H0; subst; try contradiction; try discriminate.
-  - inversion H1; subst; try contradiction; try discriminate; auto.
-  - subst. intuition.
-    + discriminate.
-    + subst. inversion H1; subst; try contradiction. intuition.
-  - inversion H1; subst; try contradiction; try discriminate; auto.
-    intuition. discriminate.
-    inversion proj_case. subst. inversion proj_case0. subst.
-    eapply apply_proj_elem_deterministic with (res1 := None) in H5; try assumption.
-    discriminate.
-  - inversion proj_case. subst.
-    inversion H1; subst; intuition; try discriminate; try contradiction.
-    inversion proj_case0. subst.
-    eapply apply_proj_elem_deterministic with (res1 := (Some (hd', Γ', p'))) in H6; try assumption.
-    inversion H6; subst.
-    specialize IHℓ with (Γ := Γ'0) (p := p'0).
-    assert (None = (Some (tl', Γ'', p''))).
-    {
-      apply IHℓ. apply normalized_cons in H. destruct H. assumption. assumption. assumption.
-    }
-    discriminate.
-  - inversion proj_case. subst.
-    inversion H1; subst; intuition; try discriminate; try contradiction.
-    inversion proj_case0. subst.
-    eapply apply_proj_elem_deterministic with (res1 := (Some (hd', Γ', p'))) in H6; try assumption.
-    inversion H6; subst.
-    inversion proj_case0. subst.
-    eapply apply_proj_elem_deterministic with (res1 := (Some (hd', Γ', p'))) in H6; try assumption.
-    inversion H6; subst.  
-    + specialize IHℓ with (Γ := Γ'0) (p := p'0).
-      assert (None = (Some (tl', Γ'', p''))).
-      {
-        apply IHℓ. apply normalized_cons in H. destruct H. assumption. assumption. assumption.
-      }
-      discriminate.
-    + inversion proj_case0. subst.
-      eapply apply_proj_elem_deterministic with (res1 := (Some (hd', Γ', p'))) in H6; try assumption.
-      inversion H6; subst.
-      specialize IHℓ with (Γ := Γ'0) (p := p'0).
-      assert ((Some (tl'0, Γ''0, p''0)) = (Some (tl', Γ'', p''))).
-      {
-        apply IHℓ. apply normalized_cons in H. destruct H. assumption. assumption. assumption.
-      }
-      inversion H8. subst.
-      (* 
-          We need to leverage Streicher'K theorem in the intensional MLTT version so that we
-          can derive the fact that all equality proofs are essentially identical, i.e.,
-
-          ∀ (A: U) ∀ (a b: A) (p q: a = b) → p = q
-
-          This holds only if equality is decidable for type A, so that A degrades into a set.
-          For non-sets that manifest complex high-order groupoid structures, adding K as an
-          axiom will break univalance axiom in HoTT.
-
-          Thus there is a paper discussing pattern matching without K in IFCP'14.
-
-          Cockx, Jesper, Dominique Devriese, and Frank Piessens. "Pattern matching without K."
-          In Proceedings of the 19th ACM SIGPLAN international conference on Functional programming. 2014.
-      *)
-      repeat f_equal. apply Eqdep.EqdepTheory.UIP.
-Qed.
-
-(*
-  @param s The schema of the relation.
-  @param Policy.context The policy context.
-  @param budget The budget for the evaluation.
-  @param prov_ctx The provenance context.
-  @param formula The formula to be evaluated.
-  @param relation The relation in which the formula is to be evaluated.
-  @param returns option A tuple containing the resulting relation, the updated policy context, the remaining
-                       budget, and the updated provenance context.
-
-  The `eval_expr_in_relation` inductive type represents the evaluation of a formula in a relation. The evalua-
-  tion is performed in the context of a given policy context and provenance context, and it may consume certain
-  amount of budget. If the evaluation is successful, the function returns `Some` with a tuple containing the
-  resulting relation, the updated policy context, the remaining budget, and the updated provenance context. If
-  the evaluation is not successful (for example, if the budget is exhausted), the function returns `None`.
-
-  FIXME: Will selection consume budget?
-*)
-Inductive eval_expr_in_relation:
-  ∀ s, Policy.context → budget → prov_ctx → formula (♭ s) → relation s →
-    option (relation s * Policy.context * budget * prov_ctx) → Prop :=
-  | E_EvalExprRelationNil: ∀ s Γ β p f r,
-      r = nil →
-      eval_expr_in_relation s Γ β p f r (Some (nil, Γ, β, p))
-  | E_EvalExprConsTrue: ∀ s Γ Γ' β β' p p' f f_denote r hd tl tl',
-      r = hd :: tl →
-      f_denote = formula_denote (♭ s) f →
-      eval_expr_in_relation s Γ β p f tl (Some (tl', Γ', β', p')) →
-      f_denote hd = true →
-      eval_expr_in_relation s Γ β p f r (Some (hd :: tl', Γ', β', p'))
-  | E_EvalExprConsFalse: ∀ s Γ Γ' β β' p p' f f_denote r hd tl tl',
-      r = hd :: tl →
-      f_denote = formula_denote (♭ s) f →
-      eval_expr_in_relation s Γ β p f tl (Some (tl', Γ', β', p')) →
-      f_denote hd = false →
-      eval_expr_in_relation s Γ β p f r (Some (tl', Γ', β', p'))
-.
-
-Lemma eval_expr_in_relation_terminate: ∀ s Γ β p f r, ∃ res,
-  eval_expr_in_relation s Γ β p f r res.
-Proof.
-  intros.
-  induction r.
-  - exists (Some (nil, Γ, β, p)). econstructor; eauto.
-  - destruct IHr. destruct x.
-    + (* Some *)
-      destruct p0 as [ [ [tl Γ'] β'] p' ].
-      destruct (formula_denote (♭ s) f a) eqn: Hdenote.
-      * exists (Some (a :: tl, Γ', β', p')). econstructor; eauto.
-      * exists (Some (tl, Γ', β', p')). econstructor; eauto.
-    + (* None *)
-      inversion H.
-Qed.
 
 (* This first creates for each tuple a `groupby_proxy` which can later be `gathered` for our convenience. *)
 Definition get_group_proxy_helper s (r: relation s) (gb_keys: groupby_list) (bounded: bounded_list s gb_keys):
@@ -1119,8 +164,6 @@ Definition get_group_proxy_helper s (r: relation s) (gb_keys: groupby_list) (bou
       end
     ) gb_keys_extracted 0.
 
-(* This function does the actual job by "gathering" all groups together. *)
-(* TODO: Perhaps we also need to take provenance into consideration? *)
 Definition get_group_proxy s (r: relation s) (gb_keys: groupby_list) (bounded: bounded_list s gb_keys):
   list (groupby_proxy (ntypes s gb_keys bounded)).
   pose (intermediate_gb_proxy := get_group_proxy_helper s r gb_keys bounded).
@@ -1149,43 +192,158 @@ Definition get_group_proxy s (r: relation s) (gb_keys: groupby_list) (bounded: b
      exact (gather a rest).
 Defined.
 
-(*
-  @param s The type of the elements in the resulting relation.
-  @param s_gb The type of the elements in the groupby_proxy list; the `groupby` keys because they are dependent types.
-  @param Policy.context The policy context.
-  @param budget The budget for the operation.
-  @param prov_ctx The provenance context.
-  @param list (groupby_proxy s_gb) The list of groupby_proxy elements.
-  @param agg_list The list of aggregation operations to be applied.
-  @param relation s The initial relation.
-  @param option (relation s * Policy.context * budget * prov_ctx) The expected result of the operation.
-  @returns Prop A proposition that is true if the operation is correctly applied, false otherwise.
-
-  The `apply_fold_on_groups` inductive type represents the application of a list of aggregation operations on a list of `groupby_proxy` elements. The operation is performed in the context of a given policy context and provenance context,
-  and it may consume a certain amount of budget. If the operation is successful, the function returns `Some` with a tuple
-  containing the resulting relation, the updated policy context, the remaining budget, and the updated provenance context.
-*)
-Inductive apply_fold_on_groups:
-  ∀ s s_gb agg, Policy.context → budget → prov_ctx → list (groupby_proxy s_gb)  → relation s →
-    option (relation (s ++ determine_agg_schema agg) * Policy.context * budget * prov_ctx) → Prop :=
+Inductive operator: Type :=
+  | operator_empty: operator
+  (* `nat` means the index of the relation it wants to access the n-th dataset inside `db`. *)
+  | operator_relation: nat → operator
+  | operator_union: operator → operator → operator
+  | operator_join: operator → operator → operator
+  | operator_project: project_list → operator → operator
+  | operator_select: expression → operator → operator
+  | operator_groupby_having: groupby_list → agg_list → expression → operator → operator
 .
 
+(*
+  @param s The schema, which is a list of tuples where each tuple contains a type and a name.
+  @param n The length of the relation to be created.
+  @param t The tuple to be repeated.
+  @return A relation of length [n] where each tuple is [t].
+
+  [tuple_of_length_n] returns a relation of length [n] where each tuple is [t]. The function
+  works by recursively appending [t] to the relation until it reaches the desired length.
+*)
+Fixpoint tuple_of_length_n s (n: nat) (t: Tuple.tuple (♭ s)): relation s :=
+match n with
+  | O => nil
+  | S n' => t :: tuple_of_length_n s n' t
+  end.
+
+Definition get_new_policy cur op: Policy.policy :=
+  match cur with
+  | ∎ => cur
+  | ℓ ⇝ p =>
+    match Policy.can_declassify_dec ℓ op with
+    | left _ => p
+    | right _ => cur
+    end
+  end.
+
+Inductive eval_expr_in_relation (s: schema) (r: relation s):
+  Policy.context → budget → prov_ctx → expression →
+    option (EResult * Policy.context * budget * prov_ctx) → Prop :=
+  | E_Eval: ∀ db db' Γ Γ' β β' p p' e env res,
+      eval_expr (⟨ db Γ β p ⟩) (relation_output s r) e (env, res) →
+      (fst (fst env)) = (⟨ db' Γ' β' p' ⟩) →
+      eval_expr_in_relation s r Γ β p e (Some (res, Γ, β, p))
+.
+
+Inductive apply_proj_in_relation (s: schema) (r: relation s) (ℓ: list (expression * string)):
+  ∀ s', Policy.context → budget → prov_ctx →
+    option (relation s' * Policy.context * budget * prov_ctx) → Prop :=
+  (* Either the projection list is empty or the relation is empty. As such, we just do nothing here. *)
+  | E_ApplyElemEmpty: ∀ s' Γ β p,
+      ℓ = nil ∨ r = nil →
+      apply_proj_in_relation s r ℓ s' Γ β p (Some (nil, Γ, β, p))
+  | E_ApplyElemErrHead: ∀ s' Γ β p hd tl,
+      ℓ = hd :: tl →
+      eval_expr_in_relation s r Γ β p (fst hd) None →
+      apply_proj_in_relation s r ℓ s' Γ β p None
+  | E_ApplyElemHeadNonRelation: ∀ s' res r' Γ Γ' β β' p p' hd tl,
+      ℓ = hd :: tl →
+      eval_expr_in_relation s r Γ β p (fst hd) (Some (res, Γ', β', p')) →
+      res ≠ EResultRelation r' →
+      apply_proj_in_relation s r ℓ s' Γ β p None
+  | E_ApplyElemErrTail: ∀ s' hd tl Γ β p,
+      ℓ = hd :: tl →
+      apply_proj_in_relation s r tl s' Γ β p None →
+      apply_proj_in_relation s r ℓ s' Γ β p None
+  | E_ApplyElemOk: ∀ s_hd s_tl Γ Γ' Γ'' β β' β'' p p' p'' hd hd' tl tl'
+                (proj_case: ℓ = hd :: tl),
+      r ≠ nil →
+      eval_expr_in_relation s r Γ β p (fst hd) (Some (EResultRelation (relation_output s_hd hd'), Γ', β', p')) →
+      Some s_tl = determine_schema s tl →
+      apply_proj_in_relation s r tl s_tl Γ' β' p' (Some (tl', Γ'', β'', p'')) →
+      (*
+        Goal:
+        (determine_schema s (project (hd :: nil)) ++
+        determine_schema s (project tl)) = determine_schema s (project ℓ)
+        -------------------------------
+        project ℓ = project (hd :: tl) by ℓ = hd :: tl with ♯
+        --–----------------------------
+        Then by determine_schema_concat we have:
+        (determine_schema s (project (hd :: nil)) ++
+        determine_schema s (project tl)) = determine_schema s (project (hd :: tl))
+        -------------------------------
+      *)
+      let col := (relation_product _ _ hd' tl') in
+        (* let col_proxy := ((determine_schema_concat s hd tl) ♯ col_tmp) in
+          col = ((eq_sym proj_case) ♯ col_proxy) → *)
+          apply_proj_in_relation s r ℓ _ Γ β p (Some (col, Γ'', β'', p''))
+.
+
+(*
+  @param s The schema of the relation.
+  @param r The relation in which the predicate is to be evaluated.
+  @param Policy.context The policy context.
+  @param budget The budget for the evaluation.
+  @param prov_ctx The provenance context.
+  @param expression The predicate to be evaluated.
+  @param option (relation s * Policy.context * budget * prov_ctx) The expected result of the evaluation.
+  @returns Prop A proposition that is true if the evaluation is correctly applied, false otherwise.
+
+  The `eval_predicate_in_relation` inductive type represents the evaluation of a predicate in a relation.
+  The evaluation is performed in the context of a given policy context and provenance context, and it may
+  consume a certain amount of budget. If the evaluation is successful, the function returns `Some` with a
+  tuple containing the resulting relation, the updated policy context, the remaining budget, and the up-
+  dated provenance context. The predicate is checked against each tuple in the relation.
+*)
+Inductive eval_predicate_in_relation (s: schema) (r: relation s):
+  Policy.context → budget → prov_ctx → expression →
+    option (relation s * Policy.context * budget * prov_ctx) → Prop :=
+  | E_EvalExprRelationNil: ∀ Γ β p e,
+      r = nil →
+      eval_predicate_in_relation s r Γ β p e (Some (nil, Γ, β, p))
+  | E_EvalExprConsTrue: ∀ db db' Γ Γ' Γ'' β β' β'' p p' p'' e env hd tl tl',
+      r = hd :: tl →
+      eval_expr (⟨ db Γ β p ⟩) (relation_output s (hd :: nil)) e (env, EResultValue BoolType true) →
+      fst (fst env) = ⟨ db' Γ' β' p' ⟩ →
+      eval_predicate_in_relation s tl Γ' β' p' e (Some (tl', Γ'', β'', p'')) →
+      eval_predicate_in_relation s r Γ β p e (Some (hd :: tl', Γ'', β'', p''))
+  | E_EvalExprConsFalse: ∀ db db' Γ Γ' Γ'' β β' β'' p p' p'' e env hd tl tl',
+      r = hd :: tl →
+      eval_expr (⟨ db Γ β p ⟩) (relation_output s (hd :: nil)) e (env, EResultValue BoolType false) →
+      fst (fst env) = ⟨ db' Γ' β' p' ⟩ →
+      eval_predicate_in_relation s tl Γ' β' p' e (Some (tl', Γ'', β'', p'')) →
+      eval_predicate_in_relation s r Γ β p e (Some (tl', Γ'', β'', p''))
+  | E_EvalError: ∀ db res v Γ β p e env hd tl,
+      r = hd :: tl →
+      eval_expr (⟨ db Γ β p ⟩) (relation_output s (hd :: nil)) e (env, res) →
+      res ≠ EResultValue BoolType v →
+      eval_predicate_in_relation s r Γ β p e None
+  | E_EvalError2: ∀ db Γ Γ' β β' p p' e env v hd tl,
+      r = hd :: tl →
+      eval_expr (⟨ db Γ β p ⟩) (relation_output s (hd :: nil)) e (env, EResultValue BoolType v) →
+      eval_predicate_in_relation s tl Γ' β' p' e None →
+      eval_predicate_in_relation s r Γ β p e None
+.
+
+(* We should invoke `eval_expr` to get the result. *)
 Inductive eval_aggregate:
-  ∀ s agg, Policy.context → budget → prov_ctx → groupby_list  → relation s →
-    option (relation (s ++ determine_agg_schema agg) * Policy.context * budget * prov_ctx) → Prop :=
-  | E_EvalAggregateNotBounded: ∀ s Γ β p gb_list agg r,
+  ∀ s s_agg, agg_list → groupby_list → Policy.context → budget → prov_ctx → relation s →
+    option (relation (s ++ s_agg) * Policy.context * budget * prov_ctx) → Prop :=
+  | E_EvalAggregateNotBounded: ∀ s s_agg Γ β p gb_list agg r,
       ¬ bounded_list s gb_list →
-      eval_aggregate s agg Γ β p gb_list r None
-  | E_EvalAggregateError: ∀ s Γ β p gb_list (bounded: bounded_list s gb_list)
+      eval_aggregate s s_agg agg gb_list Γ β p r None
+  (* | E_EvalAggregateError: ∀ s s_agg Γ β p gb_list (bounded: bounded_list s gb_list)
                        gb_proxy agg r,
       get_group_proxy s r gb_list bounded = gb_proxy →
       apply_fold_on_groups s _ agg Γ β p gb_proxy r None →
-      eval_aggregate s agg Γ β p gb_list r None
-  | E_EvalAggregateOk: ∀ s Γ Γ' β β' p p' gb_list (bounded: bounded_list s gb_list)
+      eval_aggregate s s_agg agg Γ β p gb_list r None
+  | E_EvalAggregateOk: ∀ s s_agg Γ Γ' β β' p p' gb_list (bounded: bounded_list s gb_list)
                     gb_proxy agg r r',
       get_group_proxy s r gb_list bounded = gb_proxy →
       apply_fold_on_groups s _ agg Γ β p gb_proxy r (Some (r', Γ', β', p')) →
-      eval_aggregate s agg Γ β p gb_list r (Some (r', Γ', β', p'))
+      eval_aggregate s s_agg agg Γ β p gb_list r (Some (r', Γ', β', p')) *)
 .
 
 (* 
@@ -1244,25 +402,26 @@ Inductive step_config: (config * operator) → config → Prop :=
       r = nil ∨ s = nil →
       ⟦ c (operator_project pl o) ⟧ ⇓ ⟦ c' ⟧
   (* If the operator returns a valid relation, we can then apply projection. *)
-  | E_ProjOk: ∀ c c' c'' db db' pl pl' s'
-                Γ Γ' Γ'' β β' p p' p'' r' r'' o,
+  | E_ProjOk: ∀ c c' c'' db db' pl pl' s' s''
+                Γ Γ' Γ'' β β' β'' p p' p'' r' r'' o,
       c = ⟨ db Γ β p ⟩ →
       (* We first evaluate the inner operator and get the output. *)
       ⟦ c o ⟧ ⇓ ⟦ c' ⟧ →
       (* We then destruct the output. *)
       c' = config_output (relation_output s' r') (⟨ db' Γ' β' p' ⟩) →
       s' ≠ nil ∧ r' ≠ nil →
-      (* `pl'` means a normalized project list. *)
-        normalize_project_list s' pl = project pl' →
+      (* We do a simple preprocess. *)
+      project pl' = project_list_preprocess s' pl →
+      Some s'' = determine_schema s' pl' →
         (* We then apply projection inside the environment. *)
-        apply_proj_in_relation _ r' pl' Γ p (Some (r'', Γ'', p'')) →
-        c'' = config_output (relation_output _ r'') (⟨ db' Γ'' β' p'' ⟩) →
+        apply_proj_in_relation s' r' pl' s'' Γ' β' p' (Some (r'', Γ'', β'', p'')) →
+        c'' = config_output (relation_output _ r'') (⟨ db' Γ'' β'' p'' ⟩) →
         ⟦ c (operator_project pl o) ⟧ ⇓ ⟦ c'' ⟧
   (*
      If the operator returns a valid environment, we can then apply projection. Then if the
      projection fails, we return `config_error`.
   *)
-  | E_ProjError: ∀ c c' db db' pl pl' s'
+  | E_ProjError: ∀ c c' db db' pl pl' s' s''
                 Γ Γ' β β' p p' r' o,
       c = ⟨ db Γ β p ⟩ →
       (* We first evaluate the inner operator and get the output. *)
@@ -1270,12 +429,13 @@ Inductive step_config: (config * operator) → config → Prop :=
       (* We then destruct the output. *)
       c' = config_output (relation_output s' r') (⟨ db' Γ' β' p' ⟩) →
       s' ≠ nil ∧ r' ≠ nil →
-      (* `pl'` means a normalized project list. *)
-      normalize_project_list s' pl = project pl' →
+      (* We do a simple preprocess. *)
+      project pl' = project_list_preprocess s' pl →
+      Some s'' = determine_schema s' pl' →
         (* We then apply projection inside the environment. *)
-        apply_proj_in_relation _ r' pl' Γ p None →
+        apply_proj_in_relation s' r' pl' s'' Γ β p None →
         ⟦ c (operator_project pl o) ⟧ ⇓ ⟦ config_error ⟧
-      (*
+  (*
      If the operator returns a valid environment, we can then apply projection. Then if the
      projection fails, we return `config_error`.
   *)
@@ -1284,29 +444,44 @@ Inductive step_config: (config * operator) → config → Prop :=
       (* We first evaluate the inner operator and get the output. *)
       ⟦ c o ⟧ ⇓ ⟦ config_error ⟧ →
       ⟦ c (operator_project pl o) ⟧ ⇓ ⟦ config_error ⟧
+  (*
+     If we the project list is itself wrongly typed, we return error.
+  *)
+  | E_ProjError3: ∀ c c' db db' pl pl' s'
+                Γ Γ' β β' p p' r' o,
+      c = ⟨ db Γ β p ⟩ →
+      (* We first evaluate the inner operator and get the output. *)
+      ⟦ c o ⟧ ⇓ ⟦ c' ⟧ →
+      (* We then destruct the output. *)
+      c' = config_output (relation_output s' r') (⟨ db' Γ' β' p' ⟩) →
+      s' ≠ nil ∧ r' ≠ nil →
+      (* We do a simple preprocess. *)
+      project pl' = project_list_preprocess s' pl →
+      None = determine_schema s' pl' →
+      ⟦ c (operator_project pl o) ⟧ ⇓ ⟦ config_error ⟧
   | E_SelectError: ∀ c c' db db' Γ Γ' β β' p p' s' r' o expr,
       c = ⟨ db Γ β p ⟩ →
       ⟦ c o ⟧ ⇓ ⟦ c' ⟧ →
       c' = config_output (relation_output s' r') (⟨ db' Γ' β' p' ⟩) →
-      eval_expr_in_relation s' Γ' β' p' expr r' None →
-      ⟦ c (operator_select s' expr o) ⟧ ⇓ ⟦ config_error ⟧
-  | E_SelectError2: ∀ c db Γ β p s o expr,
+      eval_predicate_in_relation s' r' Γ' β' p' expr  None →
+      ⟦ c (operator_select expr o) ⟧ ⇓ ⟦ config_error ⟧
+  | E_SelectError2: ∀ c db Γ β p o expr,
       c = ⟨ db Γ β p ⟩ →
       ⟦ c o ⟧ ⇓ ⟦ config_error ⟧ →
-      ⟦ c (operator_select s expr o) ⟧ ⇓ ⟦ config_error ⟧
+      ⟦ c (operator_select expr o) ⟧ ⇓ ⟦ config_error ⟧
   | E_SelectError3: ∀ c c' db db' Γ Γ' β β' p p' s1 s2 r' o expr,
       c = ⟨ db Γ β p ⟩ →
       ⟦ c o ⟧ ⇓ ⟦ c' ⟧ →
       c' = config_output (relation_output s2 r') (⟨ db' Γ' β' p' ⟩) →
       s1 ≠ s2 →
-      ⟦ c (operator_select s1 expr o) ⟧ ⇓ ⟦ config_error ⟧
+      ⟦ c (operator_select expr o) ⟧ ⇓ ⟦ config_error ⟧
   | E_SelectOk: ∀ c c' c'' db db' Γ Γ' Γ'' β β' β'' p p' p'' s' r' r'' o expr,
       c = ⟨ db Γ β p ⟩ →
       ⟦ c o ⟧ ⇓ ⟦ c' ⟧ →
       c' = config_output (relation_output s' r') (⟨ db' Γ' β' p' ⟩) →
-      eval_expr_in_relation s' Γ' β' p' expr r' (Some (r'', Γ'', β'', p'')) →
+      eval_predicate_in_relation s' r' Γ' β' p' expr (Some (r'', Γ'', β'', p'')) →
       c'' = config_output (relation_output s' r'') (⟨ db' Γ'' β'' p'' ⟩) →
-      ⟦ c (operator_select s' expr o)⟧ ⇓ ⟦ c'' ⟧
+      ⟦ c (operator_select expr o)⟧ ⇓ ⟦ c'' ⟧
   | E_UnionError: ∀ c c' c'' db Γ β p o1 o2,
       c = ⟨ db Γ β p ⟩ → 
       ⟦ c o1 ⟧ ⇓ ⟦ c' ⟧ →
@@ -1322,7 +497,7 @@ Inductive step_config: (config * operator) → config → Prop :=
       s1 ≠ s2 →
       ⟦ c (operator_union o1 o2) ⟧ ⇓ ⟦ config_error ⟧
   | E_UnionOk: ∀ c c' c'' db db' db'' Γ Γ' Γ'' β β' β'' p p' p'' s r' r'' o1 o2,
-      c = ⟨ db Γ β p ⟩ → 
+      c = ⟨ db Γ β p ⟩ →
       ⟦ c o1 ⟧ ⇓ ⟦ c' ⟧ →
       c' = config_output (relation_output s r') (⟨ db' Γ' β' p' ⟩) →
       ⟦ c o2 ⟧ ⇓ ⟦ c'' ⟧ →
@@ -1371,18 +546,19 @@ Inductive step_config: (config * operator) → config → Prop :=
       ⟦ c o ⟧ ⇓ ⟦ c' ⟧ →
       c' = config_output (relation_output s r) c' →
       s = nil ∨ r = nil →
-      ⟦ c (operator_groupby_having (♭ s) gl al f o) ⟧ ⇓ ⟦ c' ⟧
-  | E_AggError: ∀ c db Γ β p o s gl al f,
+      ⟦ c (operator_groupby_having gl al f o) ⟧ ⇓ ⟦ c' ⟧
+  | E_AggError: ∀ c db Γ β p o gl al f,
       c = ⟨ db Γ β p ⟩ →
       ⟦ c o ⟧ ⇓ ⟦ config_error ⟧ →
-      ⟦ c (operator_groupby_having (♭ s) gl al f o) ⟧ ⇓ ⟦ config_error ⟧
-  | E_AggError2: ∀ s c c' db db' Γ Γ' β β' p p' o r gl al f,
+      ⟦ c (operator_groupby_having gl al f o) ⟧ ⇓ ⟦ config_error ⟧
+  (* | E_AggError2: ∀ s c c' db db' Γ Γ' β β' p p' o r gl al f,
       c = ⟨ db Γ β p ⟩ →
       ⟦ c o ⟧ ⇓ ⟦ c' ⟧ →
       c' = config_output (relation_output s r) (⟨ db' Γ' β' p' ⟩) →
       s ≠ nil ∧ r ≠ nil →
-      eval_aggregate s al Γ' β' p' gl r None →
-      ⟦ c (operator_groupby_having (♭ s) gl al f o) ⟧ ⇓ ⟦ config_error ⟧
+      s_agg = determine_schema s al →
+      eval_aggregate s s_agg al gl Γ' β' p' r None →
+      ⟦ c (operator_groupby_having gl al f o) ⟧ ⇓ ⟦ config_error ⟧
   | E_AggOk: ∀ c c' c'' db db' Γ Γ' β β' p p' s al r r' o gl f,
       c = ⟨ db Γ β p ⟩ →
       ⟦ c o ⟧ ⇓ ⟦ c' ⟧ →
@@ -1390,7 +566,7 @@ Inductive step_config: (config * operator) → config → Prop :=
       s ≠ nil ∧ r ≠ nil →
       eval_aggregate s al Γ' β' p' gl r (Some (r', Γ', β', p')) →
       c'' = config_output (relation_output _ r') (⟨ db' Γ' β' p' ⟩) →
-      ⟦ c (operator_groupby_having (♭ s) gl al f o) ⟧ ⇓ ⟦ c'' ⟧
+      ⟦ c (operator_groupby_having gl al f o) ⟧ ⇓ ⟦ c'' ⟧ *)
 where "'⟦' c op '⟧' '⇓' '⟦' c' '⟧'" := (step_config (c, op) c').
 Hint Constructors step_config: core.
 
@@ -1410,7 +586,7 @@ Proof.
     + inversion H13. subst. rewrite H14 in H6. inversion H6.
     + inversion H12. subst. discriminate.
   - destruct c1; destruct c2.
-    + reflexivity.
+  + reflexivity.
     + inversion H0; subst; try discriminate.
     + inversion H; subst; try discriminate.
       * inversion H0; subst; try discriminate.
@@ -1534,122 +710,6 @@ Proof.
       * assumption.
       * assumption.
   - inversion H0; inversion H; subst; intuition; auto; subst; try discriminate.
-    + inversion H12. subst. clear H12.
-      apply (IHo (config_output (relation_output s nil) (⟨ db' Γ' β' p' ⟩))) in H13.
-      inversion H13. subst. apply inj_pair2_eq_dec in H6. subst.
-      * inversion H18; subst. exfalso. apply H2. auto. exfalso. apply H2. auto.
-      * apply list_eq_dec; apply attribute_eq_dec.
-      * assumption.
-    + inversion H12. subst. clear H12.
-      apply (IHo (config_output (relation_output nil r) (⟨ db' Γ' β' p' ⟩))) in H13.
-      inversion H13. subst. apply inj_pair2_eq_dec in H6. subst. clear H13.
-      inversion H18; subst. intuition.
-      * exfalso. apply H1. auto.
-      * exfalso. apply H1. auto.
-      * assumption.
-    + inversion H12. subst. clear H12.
-      apply (IHo (config_output (relation_output s nil) (⟨ db' Γ' β' p' ⟩))) in H13.
-      inversion H13. subst.  apply inj_pair2_eq_dec in H6. subst. clear H13.
-      * exfalso. apply H2. auto.
-      * apply list_eq_dec; apply attribute_eq_dec.
-      * assumption.
-    + inversion H12. subst. clear H12.
-      apply (IHo (config_output (relation_output nil r) (⟨ db' Γ' β' p' ⟩))) in H13; try assumption.
-      inversion H13. subst. apply inj_pair2_eq_dec in H6; subst; clear H13;
-      try (apply list_eq_dec; apply attribute_eq_dec).
-      exfalso. apply H1. auto.
-    + inversion H15. subst. clear H15.
-      apply (IHo (config_output (relation_output s nil) (⟨ db'0 Γ'0 β'0 p'0 ⟩))) in H5; try assumption.
-      inversion H5. subst. apply inj_pair2_eq_dec in H6. subst. clear H5.
-      * exfalso. apply H2. auto.
-      * apply list_eq_dec; apply attribute_eq_dec.
-    + inversion H15. subst. clear H15.
-      apply (IHo (config_output (relation_output nil r) (⟨ db'0 Γ'0 β'0 p'0 ⟩))) in H5.
-      inversion H5. subst. apply inj_pair2_eq_dec in H6. subst. clear H5.
-      * exfalso. apply H1. auto.
-      * apply list_eq_dec; apply attribute_eq_dec.
-      * assumption.
-    + inversion H15. subst. clear H15.
-      apply (IHo (config_output (relation_output s' r') (⟨ db' Γ' β' p' ⟩))) in H16.
-      inversion H16. subst. apply inj_pair2_eq_dec in H9. subst. clear H16.
-      * inversion H10. inversion H23. subst. inversion H14. inversion H24. subst.
-        clear H14. clear H24.
-        inversion H15; subst.
-        rewrite H8 in H21. inversion H21. subst. intuition; subst.
-        -- eapply apply_proj_in_relation_deterministic with (res1 := Some (r'1, Γ''0, p''0)) in H15.
-          ++ inversion H15. subst. reflexivity.
-          ++ assumption.
-          ++ assumption.
-        -- inversion H15; subst; intuition.
-          ++ discriminate.
-          ++ rewrite H8 in H21. inversion H21. subst.
-             inversion proj_case. subst. 
-             eapply apply_proj_in_relation_deterministic with (res1 := (Some (r'1, Γ''0, p''0))) in H15.
-            ** inversion H15. subst. auto.
-            ** assumption.
-            ** assumption.
-      * apply list_eq_dec; apply attribute_eq_dec.
-      * assumption.
-      (* Similar proof. *)
-    + inversion H17. subst. clear H17.
-      apply (IHo (config_output (relation_output s' r') (⟨ db' Γ' β' p' ⟩))) in H18.
-      inversion H18. subst. apply inj_pair2_eq_dec in H9. subst. clear H18.
-      * inversion H24. inversion H7. subst. clear H7.
-        inversion H9. subst.
-        -- contradiction.
-        -- rewrite H8 in H21. inversion H21. subst.
-           (* Seems to be stuck on the induction case. *)
-           inversion H10. inversion H18. subst. clear H18.
-           eapply apply_proj_in_relation_deterministic with (res1 := None) in H19.
-           ++ discriminate.
-           ++ assumption.
-           ++ assumption.
-        -- rewrite H8 in H21. inversion H21; subst.
-           inversion H10. inversion H19. subst. clear H19.
-           eapply apply_proj_in_relation_deterministic with (res1 := None) in H20.
-           ++ discriminate.
-           ++ assumption.
-           ++ assumption.
-      * apply list_eq_dec; apply attribute_eq_dec.
-      * assumption.
-    + apply (IHo config_error) in H5. discriminate. assumption.
-    + (*For this case, the proof looks similar. *)
-      inversion H15. subst. clear H15.
-      apply (IHo (config_output (relation_output s nil) (⟨ db'0 Γ'0 β'0 p'0 ⟩))) in H5.
-      inversion H5. subst. apply inj_pair2_eq_dec in H6. subst. clear H5.
-      * inversion H11. subst. inversion H4. subst. clear H4. inversion H5.
-        -- contradiction.
-        -- subst. exfalso. apply H4. auto.
-        -- subst. exfalso. apply H4. auto.
-      * apply inj_pair2_eq_dec in H6. subst. clear H5.
-        apply list_eq_dec; apply attribute_eq_dec.
-        apply list_eq_dec; apply attribute_eq_dec.
-      * assumption.
-    + inversion H15. subst. clear H15.
-      apply (IHo (config_output (relation_output nil r) (⟨ db'0 Γ'0 β'0 p'0 ⟩))) in H5.
-      inversion H5. subst. apply inj_pair2_eq_dec in H6. subst. clear H5.
-      * inversion H11. subst. inversion H4. subst. clear H4. inversion H5.
-        -- contradiction.
-        -- subst. exfalso. apply H1. auto.
-        -- exfalso. apply H1. auto.
-      * apply inj_pair2_eq_dec in H6. subst. clear H5.
-        apply list_eq_dec; apply attribute_eq_dec.
-        apply list_eq_dec; apply attribute_eq_dec.
-      * assumption.
-    + inversion H15. subst. clear H15.
-      apply (IHo (config_output (relation_output s' r') (⟨ db' Γ' β' p' ⟩))) in H16.
-      inversion H16. subst. apply inj_pair2_eq_dec in H9. subst. 
-      rewrite H8 in H19. inversion H19. subst. clear H19.
-      * inversion H11. inversion H21. inversion H7. inversion H20. subst.
-        clear H7. clear H20.
-        apply apply_proj_in_relation_deterministic with (res1 := None) in H22.
-        -- discriminate.
-        -- assumption.
-        -- assumption.
-      * apply list_eq_dec; apply attribute_eq_dec.
-      * assumption.
-    + apply (IHo config_error) in H11. discriminate. assumption.
-  - (* TODO: Proof for `select`. *)
 Admitted.
  
 (* This theorem ensures the "sanity" of the semantics to ensure that operators won't get stuck.
@@ -1712,104 +772,5 @@ Proof.
         -- exists config_error. eapply E_UnionSchemaError with (s1 := s) (s2 := s0); try eauto.
       * (* There should be no rule for constructing nested output. *)
         inversion H1; subst; try discriminate.
-      * inversion H0; subst; try discriminate.
-      * inversion H0; subst; try discriminate.
-      * inversion H1; subst; try discriminate.
-  - exists (config_output r c). eapply E_Already; reflexivity.
-  - exists config_error. eapply E_ErrorState.
-  - destruct IHo1; destruct IHo2; intuition.
-    destruct x; destruct x0.
-    + exists config_error. econstructor; try eauto.
-    + exists config_error. econstructor; try eauto.
-    + exists config_error. econstructor; try eauto.
-    + exists config_error. econstructor; try eauto.
-    + inversion H0; subst; try discriminate.
-    + inversion H0; subst; try discriminate.
-    + exists config_error; econstructor; try eauto.
-    + inversion H1; subst; try discriminate.
-    + destruct r; destruct r0; destruct x; destruct x0; subst.
-      * inversion H0; subst; try discriminate.
-      * inversion H0; subst; try discriminate.
-      * inversion H0; subst; try discriminate.
-      * inversion H1; subst; try discriminate.
-      * 
-        (* TODO: prove that this relation is decidable.  *)
-        destruct (relation_join_by_prv_terminate s s0 (natural_join_list s s0) r r0 c0 c1 b0 b1 p0 p1).
-        destruct x as[ [ [ [rjoin cjoin ] bjoin] pjoin] |].
-        -- (* x = Some *)
-          pose (rout := relation_output _ rjoin).
-          exists (config_output rout (⟨ d1 cjoin bjoin pjoin ⟩)).
-          econstructor; eauto.
-        -- exists config_error. eapply E_JoinError2; eauto.
-      * inversion H1; subst; try discriminate.
-      * inversion H1; subst; try discriminate.
-      * inversion H0; subst; try discriminate.
-      * inversion H0; subst; try discriminate.
-  - exists (config_output r c). eapply E_Already; reflexivity.
-  - intuition.
-  - intuition. destruct H0. clear H.
-    destruct x.
-    + exists config_error. eapply E_ProjError2; eauto.
-    + inversion H0; subst; try discriminate.
-    + destruct r. destruct (normalize_project_list s p) as [|pl] eqn: Hpl.
-      * inversion Hpl.
-      * destruct x.
-        -- inversion H0; subst; try discriminate.
-        -- destruct (apply_proj_in_env_terminate s (r, nil, nil, nil) pl c p0).
-           eapply normalize_is_normalized. symmetry. eauto.
-           destruct s eqn: Hs; destruct r eqn: Hr.
-           ++ exists (config_output (relation_output nil nil) (⟨ d0 c0 b0 p1 ⟩)).
-                 eapply E_ProjEmpty; eauto.
-           ++ exists (config_output (relation_output nil r) (⟨ d0 c0 b0 p1 ⟩)).
-                 eapply E_ProjEmpty; subst; eauto.
-           ++ exists (config_output (relation_output s nil) (⟨ d0 c0 b0 p1 ⟩)).
-                 eapply E_ProjEmpty; subst; eauto.
-           ++ destruct x as [ [ [e' Γ''] p'']|].
-              ** pose (r'' := env_get_relation _ e').
-                 pose (c'' := config_output (relation_output _ r'') (⟨ d0 Γ'' b0 p'' ⟩)).
-              exists c''. eapply E_ProjOk; eauto; try reflexivity.
-              split; red; intros; try discriminate.
-           ** exists config_error. eapply E_ProjError; eauto. split; intuition; discriminate.
-        -- inversion H0; subst; try discriminate.
-  - intuition. exists (config_output r c). eapply E_Already; eauto.
-  - contradiction.
-  - intuition. destruct H0. clear H.
-    destruct x.
-    + exists config_error. eapply E_SelectError2; eauto.
-    + inversion H0; subst; try discriminate.
-    + destruct r; destruct x.
-      * inversion H0; subst; try discriminate.
-      * destruct (list_eq_dec (attribute_eq_dec) s s0).
-        -- subst. destruct (eval_expr_in_relation_terminate _ c0 b0 p0 f r).
-           destruct x as [ [ [ [ r' c'] b' ] p'] | ].
-           ++ (* Some. *)
-              exists (config_output (relation_output _ r') (⟨ d0 c' b' p' ⟩)).
-              eapply E_SelectOk; eauto; try reflexivity.
-           ++ exists config_error. eapply E_SelectError; eauto.
-        -- exists config_error. eapply E_SelectError3; eauto.
-      * inversion H0; subst; try discriminate.
-  - intuition. exists (config_output r c). eapply E_Already; eauto.
-  - contradiction.
-  - intuition.
-  (* TODO: operator_groupby_having *)
+        
 Admitted.
-
-Example simple_project_list := project ((simple_atomic_expression_column 0, "foo"%string) :: nil).
-Example simple_project_list_res := normalize_project_list sample_schema simple_project_list.
-Example simple_project_list_res_correct : simple_project_list_res = project ((simple_atomic_expression_func_unary Identity (simple_atomic_expression_column 0), "foo"%string) :: @nil (simple_atomic_expression * string)).
-Proof.
-  reflexivity.
-Qed.
-
-Example simple_project_list' := project (
-  (stf_id (simple_atomic_expression_column 0), "foo"%string) ::
-  (stf_id (simple_atomic_expression_column 1), "bar"%string) ::
-  (stf_id (simple_atomic_expression_column 2), "baz"%string) ::
-  nil
-).
-
-Example simple_project_list_res' := normalize_project_list sample_schema simple_project_list'.
-Example simple_project_list_res_correct' : simple_project_list_res' = simple_project_list_res'.
-Proof.
-  reflexivity.
-Qed.
