theories/tests.v
@@ -1,4 +1,4 @@
-Require Import formula.
+Require Import expression.
 Require Import Utf8.
 
 Section Tests.
